Source/Core/node.bpl
@@ -1,77 +1,76 @@
-datatype Node<T> { Node(next: Option (Loc (Node T)), val: T) }
-type LocNode T = Loc (Node T);
+datatype Node<T> { Node(next: Option Loc, val: T) }
 
-function Between<T>(f: [One (Loc (Node T))]Node T, x: Option (Loc (Node T)), y: Option (Loc (Node T)), z: Option (Loc (Node T))): bool;
-function Avoiding<T>(f: [One (Loc (Node T))]Node T, x: Option (Loc (Node T)), y: Option (Loc (Node T)), z: Option (Loc (Node T))): bool;
-function {:inline} BetweenSet<T>(f:[One (Loc (Node T))]Node T, x: Option (Loc (Node T)), z: Option (Loc (Node T))): [Loc (Node T)]bool
+function Between<T>(f: [One Loc]Node T, x: Option Loc, y: Option Loc, z: Option Loc): bool;
+function Avoiding<T>(f: [One Loc]Node T, x: Option Loc, y: Option Loc, z: Option Loc): bool;
+function {:inline} BetweenSet<T>(f:[One Loc]Node T, x: Option Loc, z: Option Loc): [Loc]bool
 {
-  (lambda y: Loc (Node T) :: Between(f, x, Some(y), z))
+  (lambda y: Loc :: Between(f, x, Some(y), z))
 }
 
 // reflexive
-axiom {:ctor "Node"} (forall<T> f: [One (Loc (Node T))]Node T, x: Option (Loc (Node T)) :: Between(f, x, x, x));
+axiom {:ctor "Node"} (forall<T> f: [One Loc]Node T, x: Option Loc :: Between(f, x, x, x));
 
 // step
-axiom {:ctor "Node"} (forall<T> f: [One (Loc (Node T))]Node T, x: Loc (Node T) ::
+axiom {:ctor "Node"} (forall<T> f: [One Loc]Node T, x: Loc ::
   {f[One(x)]}
   Between(f, Some(x), f[One(x)]->next, f[One(x)]->next));
 
 // reach
-axiom {:ctor "Node"} (forall<T> f: [One (Loc (Node T))]Node T, x: Loc (Node T), y: Option (Loc (Node T)) ::
+axiom {:ctor "Node"} (forall<T> f: [One Loc]Node T, x: Loc, y: Option Loc ::
   {f[One(x)], Between(f, Some(x), y, y)}
   Between(f, Some(x), y, y) ==> Some(x) == y || Between(f, Some(x), f[One(x)]->next, y));
 
 // cycle
-axiom {:ctor "Node"} (forall<T> f: [One (Loc (Node T))]Node T, x: Loc (Node T), y: Option (Loc (Node T)) ::
+axiom {:ctor "Node"} (forall<T> f: [One Loc]Node T, x: Loc, y: Option Loc ::
   {f[One(x)], Between(f, Some(x), y, y)}
   f[One(x)]->next == Some(x) && Between(f, Some(x), y, y) ==> Some(x) == y);
 
 // sandwich
-axiom {:ctor "Node"} (forall<T> f: [One (Loc (Node T))]Node T, x: Option (Loc (Node T)), y: Option (Loc (Node T)) ::
+axiom {:ctor "Node"} (forall<T> f: [One Loc]Node T, x: Option Loc, y: Option Loc ::
   {Between(f, x, y, x)}
   Between(f, x, y, x) ==> x == y);
 
 // order1
-axiom {:ctor "Node"} (forall<T> f: [One (Loc (Node T))]Node T, x: Option (Loc (Node T)), y: Option (Loc (Node T)), z: Option (Loc (Node T)) ::
+axiom {:ctor "Node"} (forall<T> f: [One Loc]Node T, x: Option Loc, y: Option Loc, z: Option Loc ::
   {Between(f, x, y, y), Between(f, x, z, z)}
   Between(f, x, y, y) && Between(f, x, z, z) ==> Between(f, x, y, z) || Between(f, x, z, y));
 
 // order2
-axiom {:ctor "Node"} (forall<T> f: [One (Loc (Node T))]Node T, x: Option (Loc (Node T)), y: Option (Loc (Node T)), z: Option (Loc (Node T)) ::
+axiom {:ctor "Node"} (forall<T> f: [One Loc]Node T, x: Option Loc, y: Option Loc, z: Option Loc ::
   {Between(f, x, y, z)}
   Between(f, x, y, z) ==> Between(f, x, y, y) && Between(f, y, z, z));
 
 // transitive1
-axiom {:ctor "Node"} (forall<T> f: [One (Loc (Node T))]Node T, x: Option (Loc (Node T)), y: Option (Loc (Node T)), z: Option (Loc (Node T)) ::
+axiom {:ctor "Node"} (forall<T> f: [One Loc]Node T, x: Option Loc, y: Option Loc, z: Option Loc ::
   {Between(f, x, y, y), Between(f, y, z, z)}
   Between(f, x, y, y) && Between(f, y, z, z) ==> Between(f, x, z, z));
 
 // transitive2
-axiom {:ctor "Node"} (forall<T> f: [One (Loc (Node T))]Node T, x: Option (Loc (Node T)), y: Option (Loc (Node T)), z: Option (Loc (Node T)), w: Option (Loc (Node T)) ::
+axiom {:ctor "Node"} (forall<T> f: [One Loc]Node T, x: Option Loc, y: Option Loc, z: Option Loc, w: Option Loc ::
   {Between(f, x, y, z), Between(f, y, w, z)}
   Between(f, x, y, z) && Between(f, y, w, z) ==> Between(f, x, y, w) && Between(f, x, w, z));
 
 // transitive3
-axiom {:ctor "Node"} (forall<T> f: [One (Loc (Node T))]Node T, x: Option (Loc (Node T)), y: Option (Loc (Node T)), z: Option (Loc (Node T)), w: Option (Loc (Node T)) ::
+axiom {:ctor "Node"} (forall<T> f: [One Loc]Node T, x: Option Loc, y: Option Loc, z: Option Loc, w: Option Loc ::
   {Between(f, x, y, z), Between(f, x, w, y)}
   Between(f, x, y, z) && Between(f, x, w, y) ==> Between(f, x, w, z) && Between(f, w, y, z));
 
 // This axiom is required to deal with the incompleteness of the trigger for the reflexive axiom.
 // It cannot be proved using the rest of the axioms.
-axiom {:ctor "Node"} (forall<T> f: [One (Loc (Node T))]Node T, u: Option (Loc (Node T)), x: Option (Loc (Node T)) ::
+axiom {:ctor "Node"} (forall<T> f: [One Loc]Node T, u: Option Loc, x: Option Loc ::
   {Between(f, u, x, x)}
   Between(f, u, x, x) ==> Between(f, u, u, x));
 
 // relation between Avoiding and Between
-axiom {:ctor "Node"} (forall<T> f: [One (Loc (Node T))]Node T, x: Option (Loc (Node T)), y: Option (Loc (Node T)), z: Option (Loc (Node T)) ::
+axiom {:ctor "Node"} (forall<T> f: [One Loc]Node T, x: Option Loc, y: Option Loc, z: Option Loc ::
   {Avoiding(f, x, y, z)}
   Avoiding(f, x, y, z) <==> Between(f, x, y, z) || (Between(f, x, y, y) && !Between(f, x, z, z)));
-axiom {:ctor "Node"} (forall<T> f: [One (Loc (Node T))]Node T, x: Option (Loc (Node T)), y: Option (Loc (Node T)), z: Option (Loc (Node T)) ::
+axiom {:ctor "Node"} (forall<T> f: [One Loc]Node T, x: Option Loc, y: Option Loc, z: Option Loc ::
   {Between(f, x, y, z)}
   Between(f, x, y, z) <==> Avoiding(f, x, y, z) && Avoiding(f, x, z, z));
 
 // update
-axiom {:ctor "Node"} (forall<T> f: [One (Loc (Node T))]Node T, u: Option (Loc (Node T)), v: Option (Loc (Node T)), x: Option (Loc (Node T)), p: Loc (Node T), q: Node T ::
+axiom {:ctor "Node"} (forall<T> f: [One Loc]Node T, u: Option Loc, v: Option Loc, x: Option Loc, p: Loc, q: Node T ::
   {Avoiding(f[One(p) := q], u, v, x)}
   Avoiding(f[One(p) := q], u, v, x) <==>
     (Avoiding(f, u, v, Some(p)) && Avoiding(f, u, v, x)) || 
