Test/civl/large-samples/treiber-stack.bpl
@@ -1,39 +1,35 @@
 // RUN: %parallel-boogie -lib:base -lib:node -timeLimit:0 "%s" > "%t"
 // RUN: %diff "%s.expect" "%t"
 
-type TaggedLocNode V = TaggedLoc (Node V) Unit;
-
-datatype Treiber<V> { Treiber(top: Option (LocNode V), nodes: Map (One (LocNode V)) (Node V)) }
-type LocTreiber V = Loc (Treiber V);
-type TaggedLocTreiber V = TaggedLoc (Treiber V) Unit;
+datatype Treiber<V> { Treiber(top: Option Loc, nodes: Map (One Loc) (Node V)) }
 
 type X; // module type parameter
 
-var {:layer 2, 3} TreiberPool: Map (One (LocTreiber X)) (Vec X);
-var {:layer 0, 2} {:linear} TreiberPoolLow: Map (One (LocTreiber X)) (Treiber X);
+var {:layer 2, 3} TreiberPool: Map (One Loc) (Vec X);
+var {:layer 0, 2} {:linear} TreiberPoolLow: Map (One Loc) (Treiber X);
 
 /// Yield invariants
 
-function {:inline} Domain(ts: Map (One (LocTreiber X)) (Treiber X), loc_t: LocTreiber X): Set (One (LocNode X)) {
+function {:inline} Domain(ts: Map (One Loc) (Treiber X), loc_t: Loc): Set (One Loc) {
   ts->val[One(loc_t)]->nodes->dom
 }
 
 function {:inline} ListInDomain(t: Treiber X): bool {
-  (forall x: LocNode X:: BetweenSet(t->nodes->val, t->top, None())[x] ==> Set_Contains(t->nodes->dom, One(x)))
+  (forall x: Loc:: BetweenSet(t->nodes->val, t->top, None())[x] ==> Set_Contains(t->nodes->dom, One(x)))
 }
 
-yield invariant {:layer 1} TopInStack(loc_t: LocTreiber X);
+yield invariant {:layer 1} TopInStack(loc_t: Loc);
 preserves Map_Contains(TreiberPoolLow, One(loc_t));
 preserves (var loc_n := Map_At(TreiberPoolLow, One(loc_t))->top; loc_n is None || Set_Contains(Domain(TreiberPoolLow, loc_t), One(loc_n->t)));
-preserves (forall loc_n: LocNode X :: Set_Contains(Domain(TreiberPoolLow, loc_t), One(loc_n)) ==>
+preserves (forall loc_n: Loc :: Set_Contains(Domain(TreiberPoolLow, loc_t), One(loc_n)) ==>
               (var loc_n' := Map_At(Map_At(TreiberPoolLow, One(loc_t))->nodes, One(loc_n))->next;
                 loc_n' is None || Set_Contains(Domain(TreiberPoolLow, loc_t), One(loc_n'->t))));
 
-yield invariant {:layer 1} LocInStackOrNone(loc_t: LocTreiber X, loc_n: Option (LocNode X));
+yield invariant {:layer 1} LocInStackOrNone(loc_t: Loc, loc_n: Option Loc);
 preserves Map_Contains(TreiberPoolLow, One(loc_t));
 preserves loc_n is None || Set_Contains(Domain(TreiberPoolLow, loc_t), One(loc_n->t));
 
-yield invariant {:layer 2} ReachInStack(loc_t: LocTreiber X);
+yield invariant {:layer 2} ReachInStack(loc_t: Loc);
 preserves Map_Contains(TreiberPoolLow, One(loc_t));
 preserves (var t := Map_At(TreiberPoolLow, One(loc_t)); Between(t->nodes->val, t->top, t->top, None()));
 preserves (var t := Map_At(TreiberPoolLow, One(loc_t)); ListInDomain(t));
@@ -43,7 +39,7 @@ preserves Map_At(TreiberPool, One(loc_t)) == Abs(Map_At(TreiberPoolLow, One(loc_
 yield invariant {:layer 2} StackDom();
 preserves TreiberPool->dom == TreiberPoolLow->dom;
 
-yield invariant {:layer 2} PushLocInStack(loc_t: LocTreiber X, new_top: LocNode X, new_node: Node X, {:linear} tagged_loc: One (TaggedLocNode X));
+yield invariant {:layer 2} PushLocInStack(loc_t: Loc, new_top: Loc, new_node: Node X, {:linear} tagged_loc: One (TaggedLoc Unit));
 preserves Map_Contains(TreiberPoolLow, One(loc_t));
 preserves Set_Contains(Domain(TreiberPoolLow, loc_t), One(new_top));
 preserves tagged_loc->val == TaggedLoc(new_top, Unit());
@@ -51,10 +47,10 @@ preserves (var t := Map_At(TreiberPoolLow, One(loc_t)); Map_At(t->nodes, One(new
 
 /// Layered implementation
 
-atomic action {:layer 3} AtomicAlloc() returns ({:linear} tagged_loc: One (TaggedLocTreiber X))
+atomic action {:layer 3} AtomicAlloc() returns ({:linear} tagged_loc: One (TaggedLoc Unit))
 {
-  var one_loc_t: One (LocTreiber X);
-  var tagged_locs: Set (One (TaggedLocTreiber X));
+  var one_loc_t: One Loc;
+  var tagged_locs: Set (One (TaggedLoc Unit));
 
   call one_loc_t, tagged_locs := TaggedLocs_New(UnitSet());
   tagged_loc := One(TaggedLoc(one_loc_t->val, Unit()));
@@ -62,16 +58,16 @@ atomic action {:layer 3} AtomicAlloc() returns ({:linear} tagged_loc: One (Tagge
   assume !Map_Contains(TreiberPool, one_loc_t);
   TreiberPool := Map_Update(TreiberPool, one_loc_t, Vec_Empty());
 }
-yield procedure {:layer 2} Alloc() returns ({:linear} tagged_loc: One (TaggedLocTreiber X))
+yield procedure {:layer 2} Alloc() returns ({:linear} tagged_loc: One (TaggedLoc Unit))
 refines AtomicAlloc;
 ensures call TopInStack(tagged_loc->val->loc);
 ensures call ReachInStack(tagged_loc->val->loc);
 preserves call StackDom();
 {
-  var one_loc_t: One (LocTreiber X);
-  var tagged_locs: Set (One (TaggedLocTreiber X));
-  var top: Option (LocNode X);
-  var stack: Map (One (LocNode X)) (Node X);
+  var one_loc_t: One Loc;
+  var tagged_locs: Set (One (TaggedLoc Unit));
+  var top: Option Loc;
+  var stack: Map (One Loc) (Node X);
   var treiber: Treiber X;
 
   top := None();
@@ -85,7 +81,7 @@ preserves call StackDom();
   call {:layer 2} AbsLemma(treiber);
 }
 
-atomic action {:layer 3} AtomicPush(loc_t: LocTreiber X, x: X) returns (success: bool)
+atomic action {:layer 3} AtomicPush(loc_t: Loc, x: X) returns (success: bool)
 {
   if (*) {
     TreiberPool := Map_Update(TreiberPool, One(loc_t), Vec_Append(Map_At(TreiberPool, One(loc_t)), x));
@@ -94,15 +90,15 @@ atomic action {:layer 3} AtomicPush(loc_t: LocTreiber X, x: X) returns (success:
     success := false;
   }
 }
-yield procedure {:layer 2} {:vcs_split_on_every_assert} Push(loc_t: LocTreiber X, x: X) returns (success: bool)
+yield procedure {:layer 2} {:vcs_split_on_every_assert} Push(loc_t: Loc, x: X) returns (success: bool)
 refines AtomicPush;
 preserves call TopInStack(loc_t);
 preserves call ReachInStack(loc_t);
 preserves call StackDom();
 {
-  var old_top: Option (LocNode X);
-  var new_top: LocNode X;
-  var tagged_loc: One (TaggedLocNode X);
+  var old_top: Option Loc;
+  var new_top: Loc;
+  var tagged_loc: One (TaggedLoc Unit);
   var {:layer 2} old_treiber: Treiber X;
 
   call {:layer 2} old_treiber := Copy(TreiberPoolLow->val[One(loc_t)]);
@@ -117,7 +113,7 @@ preserves call StackDom();
   }
 }
 
-atomic action {:layer 3} AtomicPop(loc_t: LocTreiber X) returns (success: bool, x_opt: Option X)
+atomic action {:layer 3} AtomicPop(loc_t: Loc) returns (success: bool, x_opt: Option X)
 {
   var stack: Vec X;
 
@@ -135,7 +131,7 @@ atomic action {:layer 3} AtomicPop(loc_t: LocTreiber X) returns (success: bool, 
     x_opt := None();
   }
 }
-yield procedure {:layer 2} Pop(loc_t: LocTreiber X) returns (success: bool, x_opt: Option X)
+yield procedure {:layer 2} Pop(loc_t: Loc) returns (success: bool, x_opt: Option X)
 refines AtomicPop;
 preserves call TopInStack(loc_t);
 preserves call ReachInStack(loc_t);
@@ -149,16 +145,16 @@ preserves call StackDom();
   }
 }
 
-atomic action {:layer 2} AtomicAllocNode#1(loc_t: LocTreiber X, x: X)
-  returns (old_top: Option (LocNode X), new_top: LocNode X, {:linear} tagged_loc: One (TaggedLocNode X))
+atomic action {:layer 2} AtomicAllocNode#1(loc_t: Loc, x: X)
+  returns (old_top: Option Loc, new_top: Loc, {:linear} tagged_loc: One (TaggedLoc Unit))
 asserts Map_Contains(TreiberPoolLow, One(loc_t));
 {
-  var one_loc_t: One (LocTreiber X);
+  var one_loc_t: One Loc;
   var treiber: Treiber X;
-  var top: Option (LocNode X);
-  var stack: Map (One (LocNode X)) (Node X);
-  var one_loc_n: One (LocNode X);
-  var tagged_locs: Set (One (TaggedLocNode X));
+  var top: Option Loc;
+  var stack: Map (One Loc) (Node X);
+  var one_loc_n: One Loc;
+  var tagged_locs: Set (One (TaggedLoc Unit));
   
   one_loc_t := One(loc_t);
   call treiber := Map_Get(TreiberPoolLow, one_loc_t);
@@ -172,14 +168,14 @@ asserts Map_Contains(TreiberPoolLow, One(loc_t));
   treiber := Treiber(top, stack);
   call Map_Put(TreiberPoolLow, one_loc_t, treiber);
 }
-yield procedure {:layer 1} AllocNode#1(loc_t: LocTreiber X, x: X)
-  returns (old_top: Option (LocNode X), new_top: LocNode X, {:linear} tagged_loc: One (TaggedLocNode X))
+yield procedure {:layer 1} AllocNode#1(loc_t: Loc, x: X)
+  returns (old_top: Option Loc, new_top: Loc, {:linear} tagged_loc: One (TaggedLoc Unit))
 preserves call TopInStack(loc_t);
 ensures call LocInStackOrNone(loc_t, Some(new_top));
 refines AtomicAllocNode#1;
 {
-  var one_loc_n: One (LocNode X);
-  var tagged_locs: Set (One (TaggedLocNode X));
+  var one_loc_n: One Loc;
+  var tagged_locs: Set (One (TaggedLoc Unit));
 
   call old_top := ReadTopOfStack#0(loc_t);
   call LocInStackOrNone(loc_t, old_top) | TopInStack(loc_t);
@@ -190,13 +186,13 @@ refines AtomicAllocNode#1;
   call AllocNode#0(loc_t, one_loc_n, Node(old_top, x));
 }
 
-atomic action {:layer 2} AtomicPopIntermediate(loc_t: LocTreiber X) returns (success: bool, x_opt: Option X)
+atomic action {:layer 2} AtomicPopIntermediate(loc_t: Loc) returns (success: bool, x_opt: Option X)
 {
-  var one_loc_t: One (LocTreiber X);
-  var loc_n: Option (LocNode X);
+  var one_loc_t: One Loc;
+  var loc_n: Option Loc;
   var treiber: Treiber X;
-  var top: Option (LocNode X);
-  var stack: Map (One (LocNode X)) (Node X);
+  var top: Option Loc;
+  var stack: Map (One Loc) (Node X);
   var x: X;
 
   assert Map_Contains(TreiberPoolLow, One(loc_t));
@@ -220,11 +216,11 @@ atomic action {:layer 2} AtomicPopIntermediate(loc_t: LocTreiber X) returns (suc
     success := false;
   }
 }
-yield procedure {:layer 1} PopIntermediate(loc_t: LocTreiber X) returns (success: bool, x_opt: Option X)
+yield procedure {:layer 1} PopIntermediate(loc_t: Loc) returns (success: bool, x_opt: Option X)
 refines AtomicPopIntermediate;
 preserves call TopInStack(loc_t);
 {
-  var loc_n, new_loc_n: Option (LocNode X);
+  var loc_n, new_loc_n: Option Loc;
   var node: Node X;
   var x: X;
 
@@ -247,7 +243,7 @@ preserves call TopInStack(loc_t);
 
 /// Primitives
 
-yield procedure {:layer 0} LoadNode#0(loc_t: LocTreiber X, loc_n: LocNode X) returns (node: Node X);
+yield procedure {:layer 0} LoadNode#0(loc_t: Loc, loc_n: Loc) returns (node: Node X);
 refines right action {:layer 1} _
 {
   assert Map_Contains(TreiberPoolLow, One(loc_t));
@@ -255,7 +251,7 @@ refines right action {:layer 1} _
   node := TreiberPoolLow->val[One(loc_t)]->nodes->val[One(loc_n)];
 }
 
-yield procedure {:layer 0} ReadTopOfStack#0(loc_t: LocTreiber X) returns (loc_n: Option (LocNode X));
+yield procedure {:layer 0} ReadTopOfStack#0(loc_t: Loc) returns (loc_n: Option Loc);
 refines atomic action {:layer 1} _
 {
   assert Map_Contains(TreiberPoolLow, One(loc_t));
@@ -263,7 +259,7 @@ refines atomic action {:layer 1} _
 }
 
 yield procedure {:layer 0} WriteTopOfStack#0(
-  loc_t: LocTreiber X, old_loc_n: Option (LocNode X), new_loc_n: Option (LocNode X)) returns (success: bool);
+  loc_t: Loc, old_loc_n: Option Loc, new_loc_n: Option Loc) returns (success: bool);
 refines atomic action {:layer 1,2} _
 {
   assert Map_Contains(TreiberPoolLow, One(loc_t));
@@ -275,10 +271,10 @@ refines atomic action {:layer 1,2} _
   }
 }
 
-yield procedure {:layer 0} AllocNode#0(loc_t: LocTreiber X, {:linear_in} one_loc_n: One (LocNode X), node: Node X);
+yield procedure {:layer 0} AllocNode#0(loc_t: Loc, {:linear_in} one_loc_n: One Loc, node: Node X);
 refines atomic action {:layer 1} _
 {
-  var one_loc_t: One (LocTreiber X);
+  var one_loc_t: One Loc;
   var treiber: Treiber X;
 
   one_loc_t := One(loc_t);
@@ -287,7 +283,7 @@ refines atomic action {:layer 1} _
   call Map_Put(TreiberPoolLow, one_loc_t, treiber);
 }
 
-yield procedure {:layer 0} AllocTreiber#0({:linear_in} one_loc_t: One (LocTreiber X), {:linear_in} treiber: Treiber X);
+yield procedure {:layer 0} AllocTreiber#0({:linear_in} one_loc_t: One Loc, {:linear_in} treiber: Treiber X);
 refines atomic action {:layer 1,2} _
 {
   call Map_Put(TreiberPoolLow, one_loc_t, treiber);
@@ -317,7 +313,7 @@ ensures absStack == AbsDefinition(treiber');
 free ensures absStack == Abs(treiber);
 free ensures absStack == Abs(treiber');
 {
-  var loc_n: Option (LocNode X);
+  var loc_n: Option Loc;
   var n: Node X;
 
   if (treiber->top == None()) {
