Test/civl/samples/two-queues.bpl
@@ -1,29 +1,27 @@
 // RUN: %parallel-boogie -lib:base -lib:node "%s" > "%t"
 // RUN: %diff "%s.expect" "%t"
 
-datatype Queue<V> { Queue(head: LocNode V, tail: LocNode V, nodes: Map (One (LocNode V)) (Node V)) }
-
-type LocQueue V = Loc (Queue V);
+datatype Queue<V> { Queue(head: Loc, tail: Loc, nodes: Map (One (Loc)) (Node V)) }
 
 /*
 We want to model queues, a pool of (Queue int) values, and two indices pos and neg
 into that pool such that: (1) the domain of pool is linear, and
 (2) the indices pos and neg are distinct by virtue of being linear.
-We cannot model pos and neg as One (LocQueue int) because those values
+We cannot model pos and neg as One Loc because those values
 are already earmarked for the domain of queues.
-Instead, we model each of pos and neg as a One (TaggedLoc (Queue int) Unit) value,
+Instead, we model each of pos and neg as a One (TaggedLoc Unit) value,
 which allows us to achieve both goals.
 */
-var {:linear} {:layer 0, 1} queues: Map (One (LocQueue int)) (Queue int);
-var {:linear} {:layer 0, 1} pos: One (TaggedLoc (Queue int) Unit);
-var {:linear} {:layer 0, 1} neg: One (TaggedLoc (Queue int) Unit);
+var {:linear} {:layer 0, 1} queues: Map (One Loc) (Queue int);
+var {:linear} {:layer 0, 1} pos: One (TaggedLoc Unit);
+var {:linear} {:layer 0, 1} neg: One (TaggedLoc Unit);
 
 function {:inline} IsAcyclic(q: Queue int): bool
 {
     Between(q->nodes->val, Some(q->head), Some(q->tail), None())
 }
 
-function {:inline} QueueElems(q: Queue int): [LocNode int]bool
+function {:inline} QueueElems(q: Queue int): [Loc]bool
 {
     BetweenSet(q->nodes->val, Some(q->head), Some(q->tail))
 }
@@ -31,14 +29,14 @@ function {:inline} QueueElems(q: Queue int): [LocNode int]bool
 yield invariant {:layer 1} PosInv();
 preserves Map_Contains(queues, One(pos->val->loc));
 preserves (var q := Map_At(queues, One(pos->val->loc)); IsAcyclic(q) &&
-            (forall loc_n: LocNode int:: QueueElems(q)[loc_n] ==>
+            (forall loc_n: Loc:: QueueElems(q)[loc_n] ==>
                 Map_Contains(q->nodes, One(loc_n)) &&
                 (loc_n == q->tail || (var node := Map_At(q->nodes, One(loc_n)); node->val > 0))));
 
 yield invariant {:layer 1} NegInv();
 preserves Map_Contains(queues, One(neg->val->loc));
 preserves (var q := Map_At(queues, One(neg->val->loc)); IsAcyclic(q) &&
-            (forall loc_n: LocNode int:: QueueElems(q)[loc_n] ==>
+            (forall loc_n: Loc:: QueueElems(q)[loc_n] ==>
                 Map_Contains(q->nodes, One(loc_n)) &&
                 (loc_n == q->tail || (var node := Map_At(q->nodes, One(loc_n)); node->val < 0))));
 
@@ -47,7 +45,7 @@ yield procedure {:layer 1} {:vcs_split_on_every_assert} Producer(i: int)
 preserves call PosInv();
 preserves call NegInv();
 {
-    var loc: LocQueue int;
+    var loc: Loc;
 
     assert {:layer 1} pos->val->loc != neg->val->loc;
     if (i == 0) {
@@ -64,7 +62,7 @@ preserves call NegInv();
 yield procedure {:layer 1} PosConsumer()
 preserves call PosInv();
 {
-    var loc: LocQueue int;
+    var loc: Loc;
     var i: int;
 
     call loc := ReadPos();
@@ -75,7 +73,7 @@ preserves call PosInv();
 yield procedure {:layer 1} NegConsumer()
 preserves call NegInv();
 {
-    var loc: LocQueue int;
+    var loc: Loc;
     var i: int;
 
     call loc := ReadNeg();
@@ -85,24 +83,24 @@ preserves call NegInv();
 
 // Primitives
 
-yield procedure {:layer 0} ReadPos() returns (loc: LocQueue int);
+yield procedure {:layer 0} ReadPos() returns (loc: Loc);
 refines both action {:layer 1} _ {
     loc := pos->val->loc;
 }
 
-yield procedure {:layer 0} ReadNeg() returns (loc: LocQueue int);
+yield procedure {:layer 0} ReadNeg() returns (loc: Loc);
 refines both action {:layer 1} _ {
     loc := neg->val->loc;
 }
 
-yield procedure {:layer 0} Enqueue(loc_q: LocQueue int, i: int);
+yield procedure {:layer 0} Enqueue(loc_q: Loc, i: int);
 refines action {:layer 1} _
 {
-    var one_loc_q: One (LocQueue int);
+    var one_loc_q: One Loc;
     var queue: Queue int;
-    var head, tail: LocNode int;
-    var nodes: Map (One (LocNode int)) (Node int);
-    var one_loc_n, new_one_loc_n: One (LocNode int);
+    var head, tail: Loc;
+    var nodes: Map (One (Loc)) (Node int);
+    var one_loc_n, new_one_loc_n: One (Loc);
     var node: Node int;
 
     one_loc_q := One(loc_q);
@@ -121,16 +119,16 @@ refines action {:layer 1} _
     call Map_Put(queues, one_loc_q, queue);
 }
 
-yield procedure {:layer 0} Dequeue(loc_q: LocQueue int) returns (i: int);
+yield procedure {:layer 0} Dequeue(loc_q: Loc) returns (i: int);
 refines action {:layer 1} _
 {
-    var one_loc_q: One (LocQueue int);
+    var one_loc_q: One Loc;
     var queue: Queue int;
-    var head, tail: LocNode int;
-    var nodes: Map (One (LocNode int)) (Node int);
-    var one_loc_n: One (LocNode int);
+    var head, tail: Loc;
+    var nodes: Map (One (Loc)) (Node int);
+    var one_loc_n: One (Loc);
     var node: Node int;
-    var next: Option (LocNode int);
+    var next: Option (Loc);
 
     one_loc_q := One(loc_q);
     call queue := Map_Get(queues, one_loc_q);
